src/Spec/Example2.v
@@ -9,6 +9,7 @@ Require Import RelationClasses.
 Require Import Morphisms.
 Require Import List.
 Require Import Compile.
+Require Import Modules.
 
 Import ListNotations.
 
@@ -16,209 +17,251 @@ Global Set Implicit Arguments.
 Global Generalizable All Variables.
 
 
-(** Opcodes *)
+(** Opcodes and states *)
 
-Inductive opLoT : Type -> Type :=
-| Acquire : opLoT unit
-| Release : opLoT unit
-| Read : opLoT nat
-| Write : nat -> opLoT unit.
+Inductive LockOpT : Type -> Type :=
+| Acquire : LockOpT unit
+| Release : LockOpT unit
+| Read : LockOpT nat
+| Write : nat -> LockOpT unit.
 
-Inductive opMidT : Type -> Type :=
-| Inc : opMidT nat
-| Dec : opMidT nat.
+Inductive CounterOpT : Type -> Type :=
+| Inc : CounterOpT nat
+| Dec : CounterOpT nat.
 
-Variable opHiT : Type -> Type.
-
-
-(** State *)
-
-Record State := mkState {
+Record LockState := mkState {
   Value : nat;
   Lock : option nat;
 }.
 
-
-(** Semantics *)
-
-(**
- * These semantics have a built-in protocol for how threads
- * must interact with the state.  Namely, a thread cannot acquire
- * a lock that is already held; a thread cannot release another
- * thread's lock; a thread cannot read or write unless it is holding
- * the lock.
- *
- * Separately we can prove that a particular implementation
- * (e.g., ours) follows this protocol on top of a lower-level
- * semantics that does not enforce these rules.  See ExampleProtocol.v.
- *
- * So, in our framework, a concurrency protocol (e.g., rely-guarantee)
- * seems to be an extra level of refinement with semantics that codify
- * protocol violations as undefined behavior?
- *)
-
-Inductive lo_step : forall T, opLoT T -> nat -> State -> T -> State -> Prop :=
-| StepAcquire : forall tid v,
-  lo_step Acquire tid (mkState v None) tt (mkState v (Some tid))
-| StepRelease : forall tid v,
-  lo_step Release tid (mkState v (Some tid)) tt (mkState v None)
-| StepReleaseHack0 : forall tid v,
-  lo_step Release tid (mkState v None) tt (mkState v None)
-| StepReleaseHack1 : forall tid tid' v,
-  tid' <> tid ->
-  lo_step Release tid (mkState v (Some tid')) tt (mkState v (Some tid'))
-| StepRead : forall tid v,
-  lo_step Read tid (mkState v (Some tid)) v (mkState v (Some tid))
-| StepWrite : forall tid v0 v,
-  lo_step (Write v) tid (mkState v0 (Some tid)) tt (mkState v (Some tid)).
-
-Inductive mid_step : forall T, opMidT T -> nat -> State -> T -> State -> Prop :=
-| StepInc : forall tid v,
-  mid_step Inc tid (mkState v None) v (mkState (v + 1) None)
-| StepDec : forall tid v,
-  mid_step Dec tid (mkState v None) v (mkState (v - 1) None).
-
-Hint Extern 1 (lo_step _ _ _ _ _) => econstructor.
-Hint Extern 1 (mid_step _ _ _ _ _) => econstructor.
-
-Ltac step_inv :=
-  match goal with
-  | H : lo_step _ _ _ _ _ |- _ =>
-    inversion H; clear H; subst; repeat sigT_eq
-  | H : mid_step _ _ _ _ _ |- _ =>
-    inversion H; clear H; subst; repeat sigT_eq
-  end.
+Definition CounterState := nat.
 
 
-(** Implementations *)
+(** Layer definitions *)
 
-Definition inc_core : proc opLoT opMidT _ :=
-  _ <- Op Acquire;
-  v <- Op Read;
-  _ <- Op (Write (v + 1));
-  _ <- Op Release;
-  Ret v.
+Module LockAPI <: Layer.
 
-Definition dec_core : proc opLoT opMidT _ :=
-  _ <- Op Acquire;
-  v <- Op Read;
-  _ <- Op (Write (v - 1));
-  _ <- Op Release;
-  Ret v.
+  Definition opT := LockOpT.
+  Definition State := LockState.
 
-Definition compile_op T (op : opMidT T) : proc opLoT opMidT T :=
-  match op with
-  | Inc => inc_core
-  | Dec => dec_core
-  end.
+  (**
+   * These semantics have a built-in protocol for how threads
+   * must interact with the state.  Namely, a thread cannot acquire
+   * a lock that is already held; a thread cannot release another
+   * thread's lock; a thread cannot read or write unless it is holding
+   * the lock.
+   *
+   * Separately we can prove that a particular implementation
+   * (e.g., ours) follows this protocol on top of a lower-level
+   * semantics that does not enforce these rules.  See ExampleProtocol.v.
+   *
+   * So, in our framework, a concurrency protocol (e.g., rely-guarantee)
+   * seems to be an extra level of refinement with semantics that codify
+   * protocol violations as undefined behavior?
+   *)
+
+  Inductive xstep : forall T, opT T -> nat -> State -> T -> State -> Prop :=
+  | StepAcquire : forall tid v,
+    xstep Acquire tid (mkState v None) tt (mkState v (Some tid))
+  | StepRelease : forall tid v,
+    xstep Release tid (mkState v (Some tid)) tt (mkState v None)
+  | StepReleaseHack0 : forall tid v,
+    xstep Release tid (mkState v None) tt (mkState v None)
+  | StepReleaseHack1 : forall tid tid' v,
+    tid' <> tid ->
+    xstep Release tid (mkState v (Some tid')) tt (mkState v (Some tid'))
+  | StepRead : forall tid v,
+    xstep Read tid (mkState v (Some tid)) v (mkState v (Some tid))
+  | StepWrite : forall tid v0 v,
+    xstep (Write v) tid (mkState v0 (Some tid)) tt (mkState v (Some tid)).
+
+  Definition step := xstep.
+
+End LockAPI.
 
 
-(** Commutativity *)
+Module LockedCounterAPI <: Layer.
 
-Lemma acquire_right_mover :
-  right_mover lo_step Acquire.
-Proof.
-  unfold right_mover; intros.
-  repeat step_inv; try congruence; eauto.
-Qed.
+  Definition opT := CounterOpT.
+  Definition State := LockState.
 
-Lemma release_left_mover :
-  left_mover lo_step Release.
-Proof.
-  split.
-  - unfold always_enabled; intros.
-    destruct s. destruct Lock0. destruct (n == tid); subst.
-    all: eauto.
-  - unfold left_mover; intros.
+  Inductive xstep : forall T, opT T -> nat -> State -> T -> State -> Prop :=
+  | StepInc : forall tid v,
+    xstep Inc tid (mkState v None) v (mkState (v + 1) None)
+  | StepDec : forall tid v,
+    xstep Dec tid (mkState v None) v (mkState (v - 1) None).
+
+  Definition step := xstep.
+
+End LockedCounterAPI.
+
+
+Module CounterAPI <: Layer.
+
+  Definition opT := CounterOpT.
+  Definition State := CounterState.
+
+  Inductive xstep : forall T, opT T -> nat -> State -> T -> State -> Prop :=
+  | StepInc : forall tid v,
+    xstep Inc tid v v (v + 1)
+  | StepDec : forall tid v,
+    xstep Dec tid v v (v - 1).
+
+  Definition step := xstep.
+
+End CounterAPI.
+
+
+(** Using locks to get atomicity. *)
+
+Module LockingCounter <: LayerImpl LockAPI LockedCounterAPI.
+
+  Section Impl.
+
+    Variable opHiT : Type -> Type.
+
+    Definition inc_core : proc LockAPI.opT opHiT _ :=
+      _ <- Op Acquire;
+      v <- Op Read;
+      _ <- Op (Write (v + 1));
+      _ <- Op Release;
+      Ret v.
+
+    Definition dec_core : proc LockAPI.opT opHiT _ :=
+      _ <- Op Acquire;
+      v <- Op Read;
+      _ <- Op (Write (v - 1));
+      _ <- Op Release;
+      Ret v.
+
+    Definition compile_op T (op : LockedCounterAPI.opT T)
+                          : proc LockAPI.opT opHiT T :=
+      match op with
+      | Inc => inc_core
+      | Dec => dec_core
+      end.
+
+  End Impl.
+
+  Ltac step_inv :=
+    match goal with
+    | H : LockAPI.step _ _ _ _ _ |- _ =>
+      inversion H; clear H; subst; repeat sigT_eq
+    | H : LockedCounterAPI.step _ _ _ _ _ |- _ =>
+      inversion H; clear H; subst; repeat sigT_eq
+    end.
+
+  Hint Extern 1 (LockAPI.step _ _ _ _ _) => econstructor.
+  Hint Extern 1 (LockedCounterAPI.step _ _ _ _ _) => econstructor.
+
+  Lemma acquire_right_mover :
+    right_mover LockAPI.step Acquire.
+  Proof.
+    unfold right_mover; intros.
     repeat step_inv; try congruence; eauto.
-Qed.
+  Qed.
 
-Lemma read_right_mover :
-  right_mover lo_step Read.
-Proof.
-  unfold right_mover; intros.
-  repeat step_inv; try congruence; eauto.
-Qed.
+  Lemma release_left_mover :
+    left_mover LockAPI.step Release.
+  Proof.
+    split.
+    - unfold always_enabled; intros.
+      destruct s. destruct Lock0. destruct (n == tid); subst.
+      all: eauto.
+    - unfold left_mover; intros.
+      repeat step_inv; try congruence; eauto.
+  Qed.
 
-Lemma write_right_mover : forall v,
-  right_mover lo_step (Write v).
-Proof.
-  unfold right_mover; intros.
-  repeat step_inv; try congruence; eauto.
-Qed.
+  Lemma read_right_mover :
+    right_mover LockAPI.step Read.
+  Proof.
+    unfold right_mover; intros.
+    repeat step_inv; try congruence; eauto.
+  Qed.
 
-Hint Resolve acquire_right_mover.
-Hint Resolve release_left_mover.
-Hint Resolve read_right_mover.
-Hint Resolve write_right_mover.
+  Lemma write_right_mover : forall v,
+    right_mover LockAPI.step (Write v).
+  Proof.
+    unfold right_mover; intros.
+    repeat step_inv; try congruence; eauto.
+  Qed.
 
-
-(** Atomicity *)
-
-Theorem inc_atomic : forall `(rx : _ -> proc _ _ T),
-  hitrace_incl lo_step
-    (Bind (hicall compile_op Inc) rx)
-    (Bind (hicall (atomize compile_op) Inc) rx).
-Proof.
-  intros.
-  eapply hitrace_incl_atomize_ysa_hicall.
-  simpl.
-  unfold inc_core; eauto 20.
-Qed.
-
-Theorem dec_atomic : forall `(rx : _ -> proc _ _ T),
-  hitrace_incl lo_step
-    (Bind (hicall compile_op Dec) rx)
-    (Bind (hicall (atomize compile_op) Dec) rx).
-Proof.
-  intros.
-  eapply hitrace_incl_atomize_ysa_hicall.
-  simpl.
-  unfold dec_core; eauto 20.
-Qed.
+  Hint Resolve acquire_right_mover.
+  Hint Resolve release_left_mover.
+  Hint Resolve read_right_mover.
+  Hint Resolve write_right_mover.
 
 
-(** Many-thread correctness *)
+  Theorem inc_atomic : forall opHiT `(rx : _ -> proc _ _ T),
+    hitrace_incl LockAPI.step
+      (Bind (compile_op opHiT Inc) rx)
+      (Bind (atomize (compile_op opHiT) Inc) rx).
+  Proof.
+    intros.
+    eapply hitrace_incl_atomize_ysa.
+    simpl.
+    unfold inc_core; eauto 20.
+  Qed.
 
-Theorem my_compile_correct :
-  compile_correct opHiT compile_op lo_step mid_step.
-Proof.
-  unfold compile_correct; intros.
-  destruct op.
+  Theorem dec_atomic : forall opHiT `(rx : _ -> proc _ _ T),
+    hitrace_incl LockAPI.step
+      (Bind (compile_op opHiT Dec) rx)
+      (Bind (atomize (compile_op opHiT) Dec) rx).
+  Proof.
+    intros.
+    eapply hitrace_incl_atomize_ysa.
+    simpl.
+    unfold dec_core; eauto 20.
+  Qed.
 
-  + repeat atomic_exec_inv.
-    repeat step_inv.
-    simpl; intuition eauto 20.
-    simpl; intuition eauto 20.
+  Theorem my_compile_correct : forall opHiT,
+    compile_correct (compile_op opHiT) LockAPI.step LockedCounterAPI.step.
+  Proof.
+    unfold compile_correct; intros.
+    destruct op.
 
-  + repeat atomic_exec_inv.
-    repeat step_inv.
-    simpl; intuition eauto 20.
-    simpl; intuition eauto 20.
-Qed.
+    + repeat atomic_exec_inv.
+      repeat step_inv.
+      simpl; intuition eauto 20; compute; eauto.
+      simpl; intuition eauto 20; compute; eauto.
 
-Theorem my_atomize_correct :
-  atomize_correct compile_op lo_step.
-Proof.
-  unfold atomize_correct; intros.
-  destruct op.
-  + rewrite inc_atomic.
-    eapply hitrace_incl_bind_a.
-    eauto.
-  + rewrite dec_atomic.
-    eapply hitrace_incl_bind_a.
-    eauto.
-Qed.
+    + repeat atomic_exec_inv.
+      repeat step_inv.
+      simpl; intuition eauto 20; compute; eauto.
+      simpl; intuition eauto 20; compute; eauto.
+  Qed.
 
-Hint Resolve my_compile_correct.
-Hint Resolve my_atomize_correct.
+  Theorem my_atomize_correct : forall opHiT,
+    atomize_correct (compile_op opHiT) LockAPI.step.
+  Proof.
+    unfold atomize_correct; intros.
+    destruct op.
+    + rewrite inc_atomic.
+      eapply hitrace_incl_bind_a.
+      eauto.
+    + rewrite dec_atomic.
+      eapply hitrace_incl_bind_a.
+      eauto.
+  Qed.
+
+  Hint Resolve my_compile_correct.
+  Hint Resolve my_atomize_correct.
 
 
-Theorem all_traces_match :
-  forall ts1 (ts2 : @threads_state _ opHiT),
-  proc_match (compile_ok compile_op) ts1 ts2 ->
-  traces_match_ts lo_step mid_step ts1 ts2.
-Proof.
-  intros.
-  eapply compile_traces_match_ts; eauto.
-Qed.
+  Theorem all_traces_match :
+    forall opHiT ts1 (ts2 : @threads_state _ opHiT),
+    proc_match (compile_ok (compile_op opHiT)) ts1 ts2 ->
+    traces_match_ts LockAPI.step LockedCounterAPI.step ts1 ts2.
+  Proof.
+    intros.
+    eapply compile_traces_match_ts; eauto.
+  Qed.
+
+  Definition absR (s1 : LockAPI.State) (s2 : LockedCounterAPI.State) :=
+    s1 = s2.
+
+  Definition compile_ts l3opT ts :=
+    compile_ts.
+ opHiT l3opT ts.
+
+End LockingCounter.
